\documentclass[10pt]{article}
\usepackage{epsfig}
\usepackage{amsmath}
\usepackage{graphicx}
\usepackage{amssymb}


\pagestyle{empty} \setlength{\textheight}{9.5in}
\setlength{\textwidth} {6.1in} \setlength{\oddsidemargin}{0.1in}

\setlength{\evensidemargin} {0.1in}
 \setlength{\topmargin}     {-.3in}
 \setlength{\parskip} {.03 in}

\begin{document}


41 \hfill Ms. Sugrue


\begin {center}
\bf  {Proofs by Induction - Practice with \LaTeX}
\end{center}

\vspace{.1 in}


\hrule


\vspace{.2 in}


Prove  $\displaystyle{\sum_{i=1}^{n} \frac{1}{(2i-1)(2i+1)} =\frac{n}{2n+1}}$ , $\forall \hspace{.1 cm}  n  \in  \mathbb{N}$

\vspace{.3 in}

Check base case ($n=1$):


\begin{align*}
    \displaystyle \sum_{i=1}^{1} \frac{1}{(2i-1)(2i+1)} &= \frac{1}{2+1}\\
    \frac{1}{(2-1)(2+1)} &= \frac{1}{3}\\
    \frac{1}{3} &= \frac{1}{3}\\
    \end{align*}



%Notice there are lots of blank lines here.  None of those show up on my pdf file.  If you want more space on a page, you need to use \vspace{3in} to do it.






Assume
$\displaystyle{\sum_{i=1}^{k} \frac{1}{(2i-1)(2i+1)} =\frac{k}{2k+1}$ , for some $k \in \mathbb{N}}$

\vspace{.2in}

Prove
\vspace{.2in}

%The long chunk of code below is the bulk of the algebra in this proof, along with the "prove" statement.  We use this new environment, align*, so that the equations line up at the equals sign.  Check the end of this file to see what it looks like for a simpler set of equations:


\begin{align*}
   \sum_{i=1}^{k+1} \frac{1}{(2i-1)(2i+1)} &= \frac{k+1}{2(k+1)+1}\\[1em]
  \frac{1}{(2(k+1)-1)(2(k+1)+1)}+\sum_{i=1}^{k} \frac{1}{(2i-1)(2i+1)} &=\frac{k+1}{2(k+1)+1}\\[1em]
     \frac{1}{(2k+1)(2k+3)}+\frac{k}{2k+1} &= \frac{k+1}{2k+3}\\[1em]
     \frac{1}{(2k+1)(2k+3)}+\frac{k(2k+3)}{(2k+1)(2k+3)} &= \\[1em]
     \frac{2k^2+3k+1}{(2k+1)(2k+3)} &= \\[1em]
     \frac{(2k+1)(k+1)}{(2k+1)(2k+3)} &=\\[1em]
      \frac{k+1}{2k+3} &= \frac{k+1}{2k+3}\\
\end{align*}



Therefore, by the Principle of Mathematical Induction,
$\displaystyle{\sum_{i=1}^{n} \frac{1}{(2i-1)(2i+1)} =\frac{n}{2n+1}$ , $\forall \hspace{.1 cm}  n  \in  \mathbb{N}}$

\pagebreak

System of equations, aligned at their equals signs:

\begin{align*}
2x - 5y &=  8 \\
3x + 9y &=  -12
\end{align*}


{\underline{Fractions}}

\vspace{.2in}

$\frac{2}{5+x}$ (inline)

\vspace{.3in}

or bigger $\displaystyle{\frac{2}{5+x}}$

\vspace{.3in}

or big and centered.  Notice I don't need displaystyle here.

$$\frac{2}{5+x}$$

{\underline{Sigma notation}}

\vspace{.2in}

$\sum_{i=1}^{n} \left(2^{i-1}\right)$

\vspace{.2in}

Notice this is a bit small, and an inline expression that doesn't look as good as it could.  We need displaystyle again:

\vspace{.2in}

$\displaystyle{\sum_{i=1}^{n} \left(2^{i-1}\right)}$

\vspace{.2in}

or big and centered.

$$\sum_{i=1}^{n} \left(2^{i-1}\right)$$


\pagebreak
Prove  $\displaystyle{\sum_{i=1}^{n} \frac{1}{(2i-1)(2i+1)} =\frac{n}{2n+1}}$ , $\forall \hspace{.1 cm}  n  \in  \mathbb{N}$

\vspace{.3 in}

Check base case ($n=1$):


\begin{align*}
    \displaystyle \sum_{i=1}^{1} \frac{1}{(2i-1)(2i+1)} &= \frac{1}{2+1}\\
    \frac{1}{(2-1)(2+1)} &= \frac{1}{3}\\
    \frac{1}{3} &= \frac{1}{3}\\
    \end{align*}



%Notice there are lots of blank lines here.  None of those show up on my pdf file.  If you want more space on a page, you need to use \vspace{3in} to do it.






Assume
$\displaystyle{\sum_{i=1}^{k} \frac{1}{(2i-1)(2i+1)} =\frac{k}{2k+1}$ , for some $k \in \mathbb{N}}$

\vspace{.2in}

Prove
\vspace{.2in}

%The long chunk of code below is the bulk of the algebra in this proof, along with the "prove" statement.  We use this new environment, align*, so that the equations line up at the equals sign.  Check the end of this file to see what it looks like for a simpler set of equations:


\begin{align*}
   \sum_{i=1}^{k+1} \frac{1}{(2i-1)(2i+1)} &= \frac{k+1}{2(k+1)+1}\\[1em]
  \frac{1}{(2(k+1)-1)(2(k+1)+1)}+\sum_{i=1}^{k} \frac{1}{(2i-1)(2i+1)} &=\frac{k+1}{2(k+1)+1}\\[1em]
     \frac{1}{(2k+1)(2k+3)}+\frac{k}{2k+1} &= \frac{k+1}{2k+3}\\[1em]
     \frac{1}{(2k+1)(2k+3)}+\frac{k(2k+3)}{(2k+1)(2k+3)} &= \\[1em]
     \frac{2k^2+3k+1}{(2k+1)(2k+3)} &= \\[1em]
     \frac{(2k+1)(k+1)}{(2k+1)(2k+3)} &=\\[1em]
      \frac{k+1}{2k+3} &= \frac{k+1}{2k+3}\\
\end{align*}



Therefore, by the Principle of Mathematical Induction,
$\displaystyle{\sum_{i=1}^{n} \frac{1}{(2i-1)(2i+1)} =\frac{n}{2n+1}$ , $\forall \hspace{.1 cm}  n  \in  \mathbb{N}}$

\pagebreak

Prove $\displaystyle {\sum_{i=1}^{n} 5^{n-1} = \frac{5^n-1}{4}}$ , $\forall \hspace{.1 cm}  n  \in  \mathbb{N}$




\end{document}


